Extraction for Ex01a (#630) and some printing too

doc/tutorial/code/solutions_universes/Ex01a.fst
@@ -1,5 +1,11 @@
 module Ex01a
 
+// CH: Are we sure we want to get rid of all modules here
+//     (as opposed to split this between some files)?
+
+// CH: I tried to hook this up so that at least it prints something
+//     every time read or write are executed
+
 type filename = string
 
 (* canWrite is a function specifying whether or not a file f can be written *)
@@ -13,8 +19,11 @@ let canRead (f:filename) =
   canWrite f               (* writeable files are also readable *)
   || f="demo/README"  (* and so is this file *)
 
-assume val read  : f:filename{canRead f}  -> string
-assume val write : f:filename{canWrite f} -> string -> unit
+val read  : f:filename{canRead f}  -> string
+let read f  = FStar.IO.print_string ("Dummy read of file " ^ f ^ "\n"); f
+
+val write : f:filename{canWrite f} -> string -> unit
+let write f s = FStar.IO.print_string ("Dummy write of string " ^ s ^ " to file " ^ f ^ "\n")
 
   let passwd  = "demo/password"
   let readme  = "demo/README"
@@ -46,3 +55,5 @@ assume val write : f:filename{canWrite f} -> string -> unit
     let v3 = checkedRead passwd in (* this raises exception *)
     checkedWrite tmp "hello!";
     checkedWrite passwd "junk" (* this raises exception *)
+
+let main = staticChecking (); dynamicChecking ()
